src/Subst.v
@@ -3,6 +3,7 @@ Require Import Relations.
 
 Require Import MirrorCore.TypesI.
 Require Import MirrorCore.ExprI.
+Require Import MirrorCore.EnvI.
 
 Set Implicit Arguments.
 Set Strict Implicit.
@@ -26,20 +27,29 @@ Section subst.
   { substD : EnvI.env typD -> EnvI.env typD -> T -> Prop
   ; WellTyped_subst : EnvI.tenv typ -> EnvI.tenv typ -> T -> Prop
   ; substD_subst : forall u v s e t,
-                     substD u v s ->
-                     exprD u v e t = exprD u v (subst s e) t
+      substD u v s ->
+      exprD u v e t = exprD u v (subst s e) t
   ; substD_lookup : forall u v s uv e,
-                      lookup uv s = Some e ->
-                      substD u v s ->
-                      exists val, nth_error u uv = Some val /\
-                                  exprD u v e (projT1 val) = Some (projT2 val)
-  ; substD_set : forall s s' uv e,
-                   set uv e s = Some s' ->
-                   forall u v val,
-                     (substD u v s /\
-                      nth_error u uv = Some val /\
-                      exprD u v e (projT1 val) = Some (projT2 val)) <->
-                     (substD u v s')
+      lookup uv s = Some e ->
+      substD u v s ->
+      exists val,
+        nth_error u uv = Some val /\
+        exprD u v e (projT1 val) = Some (projT2 val)
+  ; WellTyped_subst_lookup : forall u v s uv e t,
+      WellTyped_subst u v s ->
+      nth_error u uv = Some t ->
+      lookup uv s = Some e ->
+      Safe_expr u v e t
+  ; WellTyped_subst_set : forall uv e s s' (u v : tenv typ),
+      WellTyped_subst u v s ->
+      set uv e s = Some s' ->
+      WellTyped_subst u v s'
+  ; substD_set : forall uv e s s' u v,
+      substD u v s' ->
+      set uv e s = Some s' ->
+      substD u v s /\
+      (forall tv, nth_error u uv = Some tv ->
+                  exprD u v e (projT1 tv) = Some (projT2 tv))
   }.
 
   Variable Subst_subst : Subst.
